08HeapMemory/HeapConversion.thy
@@ -158,6 +158,16 @@ next
     S\<^sub>h h \<V>\<^sub>h ((v\<^sub>h\<^sub>1 # \<Delta>h', p') # (\<Delta>\<^sub>h, p) # s\<^sub>h)" by simp
   ultimately show ?case by fastforce
 next
+  case (ev\<^sub>b_pushenv \<C> p v\<^sub>b \<V>\<^sub>b \<Delta>\<^sub>b s\<^sub>b)
+  then obtain h \<V>\<^sub>h' \<Delta>\<^sub>h s\<^sub>h where "\<Sigma>\<^sub>h = S\<^sub>h h \<V>\<^sub>h' ((\<Delta>\<^sub>h, Suc p) # s\<^sub>h) \<and> 
+    v\<^sub>b # \<V>\<^sub>b = map (unheap_closure h) \<V>\<^sub>h' \<and> \<Delta>\<^sub>b = map (unheap_closure h) \<Delta>\<^sub>h \<and> s\<^sub>b = unheap_stack h s\<^sub>h" 
+      by fastforce
+  moreover then obtain v\<^sub>h \<V>\<^sub>h where "\<V>\<^sub>h' = v\<^sub>h # \<V>\<^sub>h \<and> v\<^sub>b = unheap_closure h v\<^sub>h \<and> 
+    \<V>\<^sub>b = map (unheap_closure h) \<V>\<^sub>h" by fastforce
+  moreover from ev\<^sub>b_pushenv have "\<C> \<tturnstile> S\<^sub>h h (v\<^sub>h # \<V>\<^sub>h) ((\<Delta>\<^sub>h, Suc p) # s\<^sub>h) \<leadsto>\<^sub>h 
+    S\<^sub>h h \<V>\<^sub>h ((v\<^sub>h # \<Delta>\<^sub>h, p) # s\<^sub>h)" by simp
+  ultimately show ?case by fastforce
+next
   case (ev\<^sub>b_return \<C> p \<V>\<^sub>b \<Delta>\<^sub>b s\<^sub>b)
   then obtain h \<V>\<^sub>h \<Delta>\<^sub>h s\<^sub>h where "\<Sigma>\<^sub>h = S\<^sub>h h \<V>\<^sub>h ((\<Delta>\<^sub>h, Suc p) # s\<^sub>h) \<and> \<V>\<^sub>b = map (unheap_closure h) \<V>\<^sub>h \<and> 
     \<Delta>\<^sub>b = map (unheap_closure h) \<Delta>\<^sub>h \<and> s\<^sub>b = unheap_stack h s\<^sub>h" by fastforce
