08HeapMemory/HeapMemory.thy
@@ -30,6 +30,8 @@ inductive eval\<^sub>h :: "code\<^sub>b list \<Rightarrow> state\<^sub>h \<Right
     \<C> \<tturnstile> S\<^sub>h h \<V> ((\<Delta>, Suc p) # s) \<leadsto>\<^sub>h S\<^sub>h h' (v # \<V>) ((\<Delta>, p) # s)"
 | ev\<^sub>h_apply [simp]: "lookup \<C> p = Some Apply\<^sub>b \<Longrightarrow> hlookup h v\<^sub>2 = Lam\<^sub>h \<Delta>' p' \<Longrightarrow>
     \<C> \<tturnstile> S\<^sub>h h (v\<^sub>1 # v\<^sub>2 # \<V>) ((\<Delta>, Suc p) # s) \<leadsto>\<^sub>h S\<^sub>h h \<V> ((v\<^sub>1 # \<Delta>', p') # (\<Delta>, p) # s)"
+| ev\<^sub>h_pushenv [simp]: "lookup \<C> p = Some PushEnv\<^sub>b \<Longrightarrow> 
+    \<C> \<tturnstile> S\<^sub>h h (v # \<V>) ((\<Delta>, Suc p) # s) \<leadsto>\<^sub>h S\<^sub>h h \<V> ((v # \<Delta>, p) # s)"
 | ev\<^sub>h_return [simp]: "lookup \<C> p = Some Return\<^sub>b \<Longrightarrow> 
     \<C> \<tturnstile> S\<^sub>h h \<V> ((\<Delta>, Suc p) # s) \<leadsto>\<^sub>h S\<^sub>h h \<V> s"
 | ev\<^sub>h_jump [simp]: "lookup \<C> p = Some Jump\<^sub>b \<Longrightarrow> hlookup h v\<^sub>2 = Lam\<^sub>h \<Delta>' p' \<Longrightarrow>
@@ -48,6 +50,9 @@ next
 next
   case ev\<^sub>h_apply
   from ev\<^sub>h_apply(3, 1, 2) show ?case by (induction rule: eval\<^sub>h.cases) simp_all 
+next
+  case ev\<^sub>h_pushenv
+  from ev\<^sub>h_pushenv(2, 1) show ?case by (induction rule: eval\<^sub>h.cases) simp_all 
 next
   case ev\<^sub>h_return
   from ev\<^sub>h_return(2, 1) show ?case by (induction rule: eval\<^sub>h.cases) simp_all 
